wip

pulse/examples/steel_wip/ParDivWP.fst
@@ -14,7 +14,7 @@
    limitations under the License.
 *)
 module ParDivWP
-
+module T = FStar.Tactics
 (**
  * This module provides a semantic model for a combined effect of
  * divergence, state and parallel composition of atomic actions.
@@ -217,8 +217,8 @@ val as_ensures (#st:_) (#aL:Type) (#preL:st.r) (#postL: post st aL) (wpL: wp pre
 
 module C = FStar.Classical
 let wp_par (#st:st)
-           #aL (preL:st.r) (postL: post st aL) (wpL: wp preL aL postL)
-           #aR (preR:st.r) (postR: post st aR) (wpR: wp preR aR postR)
+           #aL (#preL:st.r) (#postL: post st aL) (wpL: wp preL aL postL)
+           #aR (#preR:st.r) (#postR: post st aR) (wpR: wp preR aR postR)
    : wp (preL `st.star` preR) 
         (aL & aR)
         (fun (xL, xR) -> postL xL `st.star` postR xR)
@@ -294,6 +294,14 @@ let wp_par (#st:st)
        in
        pre
 
+let bind_par (#st:st)
+           #aL (#preL:st.r) (#postL: post st aL) (wpL: wp preL aL postL)
+           #aR (#preR:st.r) (#postR: post st aR) (wpR: wp preR aR postR)
+           #a  #post (wp_k:(xL:aL -> xR:aR -> wp (postL xL `st.star` postR xR) a post))
+  : wp (preL `st.star` preR)
+       a 
+       post
+  = bind_wp (wp_par wpL wpR) (fun (xL, xR) -> wp_k xL xR)
              
 
 (** [m s c a pre post] :
@@ -308,25 +316,25 @@ let wp_par (#st:st)
  *
  *)
 noeq
-type m (s:Type u#s) (c:comm_monoid s) : (a:Type u#a) -> pre:c.r -> post:post a c -> wp pre a post -> Type =
+type m (st:st) : (a:Type u#a) -> pre:st.r -> post:post st a -> wp pre a post -> Type =
   | Ret : #a:_ 
-        -> #post:(a -> c.r) 
+        -> #post:post st a
         -> x:a
-        -> m s c a (post x) post (return_wp x post)
+        -> m st a (post x) post (return_wp x post)
         
   | Act : #a:_ 
         -> #b:_
-        -> f:action c b
-        -> #post_g:post a c 
+        -> f:action st b
+        -> #post_g:post st a
         -> #wp_g:(x:b -> wp (f.post x) a post_g)
-        -> g:(x:b -> Dv (m s c a (f.post x) post_g (wp_g x)))
-        -> m s c a f.pre post_g (bind_action f wp_g)
+        -> g:(x:b -> Dv (m st a (f.post x) post_g (wp_g x)))
+        -> m st a f.pre post_g (bind_action f wp_g)
         
-  | Par : pre0:_ -> #a0:_ -> post0:_ -> m0: m s c a0 pre0 post0 (triv_wp pre0 a0 post0) ->
-          pre1:_ -> #a1:_ -> post1:_ -> m1: m s c a1 pre1 post1 (triv_wp pre1 a1 post1) ->
-          #a:_ -> #post:_ -> wp_k:(x0:a0 -> x1:a1 -> wp (post0 x0 `c.star` post1 x1) a post)
-               -> k:(x0:a0 -> x1:a1 -> Dv (m s c a (c.star (post0 x0) (post1 x1)) post (wp_k x0 x1))) ->
-          m s c a (c.star pre0 pre1) post (bind_par post0 post1 wp_k)
+  | Par : preL:_ -> aL:_ -> postL:_ -> wpL:wp preL aL postL -> mL: m st aL preL postL wpL ->
+          preR:_ -> aR:_ -> postR:_ -> wpR:wp preR aR postR -> mR: m st aR preR postR wpR ->
+          #a:_ -> post:_ -> wp_k:(xL:aL -> xR:aR -> wp (postL xL `st.star` postR xR) a post)
+          -> k:(xL:aL -> xR:aR -> Dv (m st a (postL xL `st.star` postR xR) post (wp_k xL xR))) ->
+          m st a (st.star preL preR) post (bind_par wpL wpR wp_k)
 
 
 /// We assume a stream of booleans for the semantics given below
@@ -343,243 +351,282 @@ val bools : nat -> bool
 ///      until it returns with a result and final state.
 
 
-let frame_post #s (#c:comm_monoid s) #a (post:post a c) (frame:c.r) = fun x -> post x `c.star` frame
-
-///
-/// [step_result s c a q frame]:
-///   The result of evaluating a single step of a program
-///   - s, c: The state and its monoid
-///   - a : the result type
-///   - q : the postcondition to be satisfied after fully reducing the programs
-///   - frame: a framed assertion to carry through the proof
 noeq
-type step_result s (c:comm_monoid s) a (q:post a c) (frame:c.r) (k:wp_post a q) =
+type step_result (#st:st) a (q:post st a) (frame:st.r) (k:wp_post a q) =
   | Step: p:_ -> //precondition of the reduct
           wp:wp p a q ->
-          m s c a p q wp -> //the reduct
-          state:rs (p `c.star` frame) { 
-            (assume (c.interp p state);
-             wp k state)
+          m st a p q wp -> //the reduct
+          state:rs (p `st.star` frame) { 
+             wp k state
           } ->
           //the next state, satisfying the precondition of the reduct
           nat -> //position in the stream of booleans (less important)
-          step_result s c a q frame k
+          step_result a q frame k
 
-let triv_post #s (#c:comm_monoid s) (a:Type) (post:post a c) : wp_post a post = fun _ _ -> True
+let triv_post #st (a:Type) (p:post st a) : wp_post a p = 
+  let k (x:a) : rs_prop (p x) = 
+    let p : rs_prop' (p x) = fun s -> True in
+    p
+  in
+  k
 
+#push-options "--query_stats"
+#push-options "--z3rlimit_factor 10 --max_fuel 1 --max_ifuel 2 --initial_ifuel 2"
 /// [step i f frame state]: Reduces a single step of [f], while framing
 /// the assertion [frame]
-let rec step #s #c (i:nat) #pre #a #post 
-             (frame:c.r)
+let rec step #st (i:nat) #pre #a #post 
+             (frame:st.r)
              (#wp:wp pre a post)
-             (f:m s c a pre post wp)
+             (f:m st a pre post wp)
              (k:wp_post a post)
-             (state:s)
-  : Div (step_result s c a post frame k)
+             (state:st.s)
+  : Div (step_result a post frame k)
         (requires
-          c.interp (pre `c.star` frame) state /\
-          c.interp pre state /\
+          st.interp (pre `st.star` frame) state /\
+          st.interp pre state /\
           wp k state)
         (ensures fun _ -> True)
   = match f with
     | Ret x ->
-        //Nothing to do, just return
-        Step (post x) wp (Ret x) state i
+        admit()
+        // //Nothing to do, just return
+        // Step (post x) wp (Ret x) state i
     
     | Act act1 #post_g #wp_g g ->
-        //Evaluate the action and return the continuation as the reduct
-        let (| b, state' |) = act1.sem frame state in
-        assert (c.interp (act1.post b `c.star` frame) state');
-        assert (wp == bind_action act1 wp_g);
-        assert (bind_action act1 wp_g k state);
-        assume (c.interp (act1.post b) state');
-        let (| emp_b, emp_state' |) = act1.sem c.emp state in
-        assume (b == emp_b);
-        assume (emp_state' == state');
-        assert (wp_g b k state');
-        Step (act1.post b) (wp_g b) (g b) state' i
-    
-    | Par pre0 post0 (Ret x0)
-          pre1 post1 (Ret x1)
-          wp_k k ->
-        assert (wp == bind_par post0 post1 wp_k);
-        //If both sides of a `Par` have returned
-        //then step to the continuation
-        Step (post0 x0 `c.star` post1 x1)
-             (wp_k x0 x1) 
-             (k x0 x1) 
-             state
-             i
+        admit()
+        // //Evaluate the action and return the continuation as the reduct
+        // let b, state' = act1.sem state in
+        // assert (st.interp (act1.pre `st.star` frame) state);        
+        // assert (st.interp (act1.post b `st.star` frame) state');
+        // assert (wp == bind_action act1 wp_g);
+        // assert (bind_action act1 wp_g k state);
+        // assert (st.interp (act1.post b) state');
+        // assert (wp_g b k state');
+        // Step (act1.post b) (wp_g b) (g b) state' i
 
-    
-    | Par pre0 #a0 post0 m0
-          pre1 #a1 post1 m1
-          #a #post wp_kont kont ->
-        assert (wp == bind_par post0 post1 wp_kont);      
-        assert (bind_par #_ #_ #(c.star pre0 pre1) post0 post1 wp_kont k state );
-        assert (triv_wp #_ #_ (pre0 `c.star` (pre1 `c.star` frame)) a0 post0 (triv_post a0 post0) state);
+    | Par preL aL postL wpL (Ret xL)
+          preR aR postR wpR (Ret xR)
+          post wp_k kk -> 
+      admit();
+      assert (wpL == return_wp xL postL);
+      assert (wpR == return_wp xR postR);      
+      assert (wp == bind_par wpL wpR wp_k);
+      assert (wp k state);
+      let sL, rest = st.split preL state in
+      let sR, rest = st.split preR state in
+      let s' = st.join (sL, st.join (sR, rest)) in
+      assert (st.interp (postL xL) sL);
+      assert (st.interp (postR xR) sR);      
+      assume (s' == state);
+      assert (st.interp (postL xL `st.star` postR xR) s');
+      Step (postL xL `st.star` postR xR)
+           (wp_k xL xR) 
+           (kk xL xR) 
+           state
+           i
 
-        //Otherwise, sample a boolean and choose to go left or right to pick
-        //the next command to reduce
-        //The two sides are symmetric
-        if bools i
-        then let Step pre0' wp0' m0' state' j =
-                 //Notice that, inductively, we instantiate the frame extending
-                 //it to include the precondition of the other side of the par
-                 assert (c.interp (pre0 `c.star` (pre1 `c.star` frame)) state);
-                 assume (c.interp pre0 state);
-                 step (i + 1) (pre1 `c.star` frame) m0 (triv_post a0 post0) state in
-             Step (pre0' `c.star` pre1) 
-                  (bind_par post0 post1 wp_kont)
-                  (Par pre0' post0 m0' pre1 post1 m1 wp_kont kont)
-                  state'
-                  j
-        else admit()
+    | Par preL aL postL wpL mL
+          preR aR postR wpR mR
+          post wp_kont kont -> 
+      assert (wp == bind_par wpL wpR wp_kont);
+      
+      //Otherwise, sample a boolean and choose to go left or right to pick
+      //the next command to reduce
+      //The two sides are symmetric
+      if bools i
+      then let Step preL' wpL' mL' state' j =
+             //Notice that, inductively, we instantiate the frame extending
+             //it to include the precondition of the other side of the par
+             assert (st.interp (preL `st.star` (preR `st.star` frame)) state);
+             assert (as_requires wpL (fst (st.split preL state)));
+             assert (as_requires wpL state);
+             assume (wpL (triv_post aL postL) state);
+             step (i + 1) (preR `st.star` frame) mL (triv_post aL postL) state
+           in             
+           assert (wpL' (triv_post aL postL) state');
+           assume (as_requires wpL' state');
+           assert (st.interp (preR `st.star` (preL `st.star` frame)) state);           
+           assert (as_requires wpR (fst (st.split preR (snd (st.split preL state)))));
+           assume (as_requires wpR state);
+           assume (wpR (triv_post aR postR) state');
+           assume (as_requires wpR state');
+
+           let sL, rest = st.split preL' state' in
+           let sR, rest = st.split preR rest in
+           
+           assume 
+           (as_requires wpL' sL /\
+            as_requires wpR sR /\
+            (forall xL sL' xR sR'.
+                  let s1 = st.join (sL', st.join(sR',rest)) in
+                  st.interp (postL xL) sL' /\
+                  st.interp (postR xR) sR' /\                 
+                  st.interp (postL xL `st.star` postR xR) s1 ==>
+                  wp_kont xL xR k s1));
+           assert (bind_par wpL' wpR wp_kont k state');
+           admit();
+           Step (preL' `st.star` preR)
+                (bind_par wpL' wpR wp_kont)
+                (Par preL' aL postL wpL' mL'
+                     preR  aR postR wpR  mR
+                     post wp_kont kont)
+                state'
+                j
+      else admit()
+      
+//                  assume (c.interp pre0 state);
+//                  step (i + 1) (pre1 `c.star` frame) m0 (triv_post a0 post0) state in
+//              Step (pre0' `c.star` pre1) 
+//                   (bind_par post0 post1 wp_kont)
+//                   (Par pre0' post0 m0' pre1 post1 m1 wp_kont kont)
+//                   state'
+//                   j
+//         else admit()
         
-//         let Step pre1' m1' state' j =
-//                  step (i + 1) m1 (pre0 `c.star` frame) state in
-//              Step (pre0 `c.star` pre1') (Par pre0 post0 m0 pre1' post1 m1' k) state' j
+// //         let Step pre1' m1' state' j =
+// //                  step (i + 1) m1 (pre0 `c.star` frame) state in
+// //              Step (pre0 `c.star` pre1') (Par pre0 post0 m0 pre1' post1 m1' k) state' j
 
-// // (**
-// //  * [run i f state]: Top-level driver that repeatedly invokes [step]
-// //  *
-// //  * The type of [run] is the main theorem. It states that it is sound
-// //  * to interpret the indices of `m` as a Hoare triple in a
-// //  * partial-correctness semantics
-// //  *
-// //  *)
-// // let rec run #s #c (i:nat) #pre #a #post (f:m s c a pre post) (state:s)
-// //   : Div (a & s)
-// //     (requires
-// //       c.interp pre state)
-// //     (ensures fun (x, state') ->
-// //       c.interp (post x) state')
-// //   = match f with
-// //     | Ret x -> x, state
-// //     | _ ->
-// //       let Step pre' f' state' j = step i f c.emp state in
-// //       run j f' state'
+// // // (**
+// // //  * [run i f state]: Top-level driver that repeatedly invokes [step]
+// // //  *
+// // //  * The type of [run] is the main theorem. It states that it is sound
+// // //  * to interpret the indices of `m` as a Hoare triple in a
+// // //  * partial-correctness semantics
+// // //  *
+// // //  *)
+// // // let rec run #s #c (i:nat) #pre #a #post (f:m s c a pre post) (state:s)
+// // //   : Div (a & s)
+// // //     (requires
+// // //       c.interp pre state)
+// // //     (ensures fun (x, state') ->
+// // //       c.interp (post x) state')
+// // //   = match f with
+// // //     | Ret x -> x, state
+// // //     | _ ->
+// // //       let Step pre' f' state' j = step i f c.emp state in
+// // //       run j f' state'
 
-// // ////////////////////////////////////////////////////////////////////////////////
-// // //The rest of this module shows how this semantic can be packaged up as an
-// // //effect in F*
-// // ////////////////////////////////////////////////////////////////////////////////
+// // // ////////////////////////////////////////////////////////////////////////////////
+// // // //The rest of this module shows how this semantic can be packaged up as an
+// // // //effect in F*
+// // // ////////////////////////////////////////////////////////////////////////////////
 
-// // (** [eff a pre post] : The representation-type for a layered effect
-// //  *
-// //  *   - Note, we'll probably have to add a thunk to make it work with
-// //  *     the current implementation but that's a detail
-// //  *)
-// // let eff #s (#c:comm_monoid s) a (pre:c.r) (post: a -> c.r) =
-// //   m s c a pre post
+// // // (** [eff a pre post] : The representation-type for a layered effect
+// // //  *
+// // //  *   - Note, we'll probably have to add a thunk to make it work with
+// // //  *     the current implementation but that's a detail
+// // //  *)
+// // // let eff #s (#c:comm_monoid s) a (pre:c.r) (post: a -> c.r) =
+// // //   m s c a pre post
 
-// // /// eff is a monad: we give a return and bind for it, though we don't
-// // /// prove the monad laws
-
-
-// // (** [return]: easy, just use Ret *)
-// // let return #s (#c:comm_monoid s) #a (x:a) (post:a -> c.r)
-// //   : eff a (post x) post
-// //   = Ret x
-
-// // (**
-// //  * [bind]: sequential composition works by pushing `g` into the continuation
-// //  * at each node, finally applying it at the terminal `Ret`
-// //  *)
-// // let rec bind #s (#c:comm_monoid s) #a #b (#p:c.r) (#q:a -> c.r) (#r:b -> c.r)
-// //              (f:eff a p q)
-// //              (g: (x:a -> eff b (q x) r))
-// //   : Dv (eff b p r)
-// //   = match f with
-// //     | Ret x -> g x
-// //     | Act act k ->
-// //       Act act (fun x -> bind (k x) g)
-// //     | Par pre0 post0 l
-// //           pre1 post1 r
-// //           k ->
-// //       Par pre0 post0 l pre1 post1 r (fun x0 x1 -> bind (k x0 x1) g)
-
-// // (**
-// //  * [par]: Parallel composition
-// //  * Works by just using the `Par` node and `Ret` as its continuation
-// //  **)
-// // let par #s (#c:comm_monoid s)
-// //         #a0 #p0 #q0 (m0:eff a0 p0 q0)
-// //         #a1 #p1 #q1 (m1:eff a1 p1 q1)
-// //  : eff (a0 & a1) (p0 `c.star` p1) (fun (x0, x1) -> q0 x0 `c.star` q1 x1)
-// //  = Par p0 q0 m0
-// //        p1 q1 m1
-// //        #_ #(fun (x0, x1) -> c.star (q0 x0) (q1 x1)) (fun x0 x1 -> Ret (x0, x1))
+// // // /// eff is a monad: we give a return and bind for it, though we don't
+// // // /// prove the monad laws
 
 
-// // /// Now for an instantiation of the state with a heap
-// // /// just to demonstrate how that would go
+// // // (** [return]: easy, just use Ret *)
+// // // let return #s (#c:comm_monoid s) #a (x:a) (post:a -> c.r)
+// // //   : eff a (post x) post
+// // //   = Ret x
 
-// // /// Heaps are usually in a universe higher than the values they store
-// // /// Pick it in universe 1
-// // assume val heap : Type u#1
+// // // (**
+// // //  * [bind]: sequential composition works by pushing `g` into the continuation
+// // //  * at each node, finally applying it at the terminal `Ret`
+// // //  *)
+// // // let rec bind #s (#c:comm_monoid s) #a #b (#p:c.r) (#q:a -> c.r) (#r:b -> c.r)
+// // //              (f:eff a p q)
+// // //              (g: (x:a -> eff b (q x) r))
+// // //   : Dv (eff b p r)
+// // //   = match f with
+// // //     | Ret x -> g x
+// // //     | Act act k ->
+// // //       Act act (fun x -> bind (k x) g)
+// // //     | Par pre0 post0 l
+// // //           pre1 post1 r
+// // //           k ->
+// // //       Par pre0 post0 l pre1 post1 r (fun x0 x1 -> bind (k x0 x1) g)
 
-// // /// Assume some monoid of heap assertions
-// // assume val hm : comm_monoid heap
-
-// // /// For this demo, we'll also assume that this assertions are affine
-// // ///  i.e., it's ok to forget some properties of the heap
-// // assume val hm_affine (r0 r1:hm.r) (h:heap)
-// //   : Lemma (hm.interp (r0 `hm.star` r1) h ==>
-// //            hm.interp r0 h)
-
-// // /// Here's a ref type
-// // assume val ref : Type u#0 -> Type u#0
-
-// // /// And two atomic heap assertions
-// // assume val ptr_live (r:ref 'a) : hm.r
-// // assume val pts_to (r:ref 'a) (x:'a) : hm.r
-
-// // /// sel: Selected a reference from a heap, when that ref is live
-// // assume val sel (x:ref 'a) (h:heap{hm.interp (ptr_live x) h})
-// //   : Tot 'a
-// // /// this tells us that sel is frameable
-// // assume val sel_ok (x:ref 'a) (h:heap) (frame:hm.r)
-// //   : Lemma (hm.interp (ptr_live x `hm.star` frame) h ==>
-// //            (hm_affine (ptr_live x) frame h;
-// //             let v = sel x h in
-// //             hm.interp (pts_to x v `hm.star` frame) h))
+// // // (**
+// // //  * [par]: Parallel composition
+// // //  * Works by just using the `Par` node and `Ret` as its continuation
+// // //  **)
+// // // let par #s (#c:comm_monoid s)
+// // //         #a0 #p0 #q0 (m0:eff a0 p0 q0)
+// // //         #a1 #p1 #q1 (m1:eff a1 p1 q1)
+// // //  : eff (a0 & a1) (p0 `c.star` p1) (fun (x0, x1) -> q0 x0 `c.star` q1 x1)
+// // //  = Par p0 q0 m0
+// // //        p1 q1 m1
+// // //        #_ #(fun (x0, x1) -> c.star (q0 x0) (q1 x1)) (fun x0 x1 -> Ret (x0, x1))
 
 
-// // /// upd: updates a heap at a given reference, when the heap contains it
-// // assume val upd (x:ref 'a) (v:'a) (h:heap{hm.interp (ptr_live x) h})
-// //   : Tot heap
-// // /// and upd is frameable too
-// // assume val upd_ok (x:ref 'a) (v:'a) (h:heap) (frame:hm.r)
-// //   : Lemma (hm.interp (ptr_live x `hm.star` frame) h ==>
-// //            (hm_affine (ptr_live x) frame h;
-// //             let h' = upd x v h in
-// //             hm.interp (pts_to x v `hm.star` frame) h'))
+// // // /// Now for an instantiation of the state with a heap
+// // // /// just to demonstrate how that would go
 
-// // /// Here's a sample action for dereference
-// // let (!) (x:ref 'a)
-// //   : eff 'a (ptr_live x) (fun v -> pts_to x v)
-// //   = let act : action hm 'a =
-// //     {
-// //       pre = ptr_live x;
-// //       post = pts_to x;
-// //       sem = (fun frame h0 ->
-// //         hm_affine (ptr_live x) frame h0;
-// //         sel_ok x h0 frame;
-// //         (| sel x h0, h0 |))
-// //     } in
-// //     Act act Ret
+// // // /// Heaps are usually in a universe higher than the values they store
+// // // /// Pick it in universe 1
+// // // assume val heap : Type u#1
 
-// // /// And a sample action for assignment
-// // let (:=) (x:ref 'a) (v:'a)
-// //   : eff unit (ptr_live x) (fun _ -> pts_to x v)
-// //   = let act : action hm unit =
-// //     {
-// //       pre = ptr_live x;
-// //       post = (fun _ -> pts_to x v);
-// //       sem = (fun frame h0 ->
-// //         hm_affine (ptr_live x) frame h0;
-// //         upd_ok x v h0 frame;
-// //         (| (), upd x v h0 |))
-// //     } in
-// //     Act act Ret
+// // // /// Assume some monoid of heap assertions
+// // // assume val hm : comm_monoid heap
+
+// // // /// For this demo, we'll also assume that this assertions are affine
+// // // ///  i.e., it's ok to forget some properties of the heap
+// // // assume val hm_affine (r0 r1:hm.r) (h:heap)
+// // //   : Lemma (hm.interp (r0 `hm.star` r1) h ==>
+// // //            hm.interp r0 h)
+
+// // // /// Here's a ref type
+// // // assume val ref : Type u#0 -> Type u#0
+
+// // // /// And two atomic heap assertions
+// // // assume val ptr_live (r:ref 'a) : hm.r
+// // // assume val pts_to (r:ref 'a) (x:'a) : hm.r
+
+// // // /// sel: Selected a reference from a heap, when that ref is live
+// // // assume val sel (x:ref 'a) (h:heap{hm.interp (ptr_live x) h})
+// // //   : Tot 'a
+// // // /// this tells us that sel is frameable
+// // // assume val sel_ok (x:ref 'a) (h:heap) (frame:hm.r)
+// // //   : Lemma (hm.interp (ptr_live x `hm.star` frame) h ==>
+// // //            (hm_affine (ptr_live x) frame h;
+// // //             let v = sel x h in
+// // //             hm.interp (pts_to x v `hm.star` frame) h))
+
+
+// // // /// upd: updates a heap at a given reference, when the heap contains it
+// // // assume val upd (x:ref 'a) (v:'a) (h:heap{hm.interp (ptr_live x) h})
+// // //   : Tot heap
+// // // /// and upd is frameable too
+// // // assume val upd_ok (x:ref 'a) (v:'a) (h:heap) (frame:hm.r)
+// // //   : Lemma (hm.interp (ptr_live x `hm.star` frame) h ==>
+// // //            (hm_affine (ptr_live x) frame h;
+// // //             let h' = upd x v h in
+// // //             hm.interp (pts_to x v `hm.star` frame) h'))
+
+// // // /// Here's a sample action for dereference
+// // // let (!) (x:ref 'a)
+// // //   : eff 'a (ptr_live x) (fun v -> pts_to x v)
+// // //   = let act : action hm 'a =
+// // //     {
+// // //       pre = ptr_live x;
+// // //       post = pts_to x;
+// // //       sem = (fun frame h0 ->
+// // //         hm_affine (ptr_live x) frame h0;
+// // //         sel_ok x h0 frame;
+// // //         (| sel x h0, h0 |))
+// // //     } in
+// // //     Act act Ret
+
+// // // /// And a sample action for assignment
+// // // let (:=) (x:ref 'a) (v:'a)
+// // //   : eff unit (ptr_live x) (fun _ -> pts_to x v)
+// // //   = let act : action hm unit =
+// // //     {
+// // //       pre = ptr_live x;
+// // //       post = (fun _ -> pts_to x v);
+// // //       sem = (fun frame h0 ->
+// // //         hm_affine (ptr_live x) frame h0;
+// // //         upd_ok x v h0 frame;
+// // //         (| (), upd x v h0 |))
+// // //     } in
+// // //     Act act Ret
